chapter02-spec/exercises/exercise02.dfy
@@ -5,7 +5,7 @@
 // Take another little detour to implementation-land by writing a method
 // `test_prime` that implements IsPrime with an imperative while() loop.
 
-predicate divides(factor:nat, candidate:nat)
+predicate method divides(factor:nat, candidate:nat)
   requires 1<=factor
 {
   candidate % factor == 0
@@ -17,13 +17,33 @@ predicate IsPrime(candidate:nat)
   && ( forall factor :: 1 < factor < candidate ==> !divides(factor, candidate) )
 }
 
+/*
+What does it mean by
+"return statement is not allowed in this context (because it is guarded by a specification-only expression)"
+*/
 // Convincing the proof to go through requires adding
 // a loop invariant and a triggering assert.
 method test_prime(candidate:nat) returns (result:bool)
   requires 1<candidate
   ensures result == IsPrime(candidate)
 {
-  // Fill in the body.
+  if (1 < candidate) {
+    var factor := 2;
+
+    while (factor < candidate)
+      invariant forall factor1:nat | 1 < factor1 < factor :: !divides(factor1, candidate)
+    {
+      var divides_result := divides(factor, candidate);
+      if (divides_result) {
+        return false;
+      }
+      factor := factor + 1;
+    }
+    assert IsPrime(candidate);
+    return true;
+  } else {
+    result := false;
+  }
 }
 
 method Main()
