chapter02-spec/exercises/exercise03.dfy
@@ -15,7 +15,20 @@ predicate IsSorted(seqint:seq<int>)
 method merge_sort(input:seq<int>) returns (output:seq<int>)
   ensures IsSorted(output)
 {
-  // Supply the body.
+  if |input| <= 1 {
+    output := input;
+  } else {
+    var pivotIndex := |input| / 2;
+    var left := input[..pivotIndex];
+    var right := input[pivotIndex..];
+    if left!=[] {
+      left := merge_sort(left);
+    }
+    if right!=[] {
+      right := merge_sort(right);
+    }
+    output := merge(left, right);
+  }
 }
 
 method merge(seqa:seq<int>, seqb:seq<int>) returns (output:seq<int>)
@@ -23,5 +36,23 @@ method merge(seqa:seq<int>, seqb:seq<int>) returns (output:seq<int>)
   requires IsSorted(seqb)
   ensures IsSorted(output)
 {
-  // Supply the body.
+  var idxa := 0;
+  var idxb := 0;
+  output := [];
+  while idxa < |seqa| || idxb < |seqb|
+    invariant idxa <= |seqa|
+    invariant idxb <= |seqb|
+    invariant |output| > 0 && idxa < |seqa| ==> output[|output| - 1] <= seqa[idxa]
+    invariant |output| > 0 && idxb < |seqb| ==> output[|output| - 1] <= seqb[idxb]
+    invariant IsSorted(output)
+    decreases |seqa| - idxa + |seqb| - idxb
+  {
+    if idxa == |seqa| || (idxb < |seqb| && seqa[idxa] >= seqb[idxb]) {
+      output := output + [seqb[idxb]];
+      idxb := idxb + 1;
+    } else {
+      output := output + [seqa[idxa]];
+      idxa := idxa + 1;
+    }
+  }
 }
